add semantics clocking constraints --> is everything needed when clocks are not generalized?

Clocks.v
@@ -1,6 +1,9 @@
 Require Import Velus.Common.
 Require Import List.
 
+Require Import Morphisms.
+Import Permutation.
+
 Module Type CLOCKS
        (Ids : IDS).
 
@@ -8,7 +11,7 @@ Module Type CLOCKS
 
   Inductive clock : Type :=
   | Cbase : clock                            (* base clock *)
-  | Con   : clock -> ident -> bool -> clock.       (* subclock *)
+  | Con   : clock -> ident -> bool -> clock. (* subclock *)
 
   Inductive Is_free_in_clock : ident -> clock -> Prop :=
   | FreeCon1:
@@ -18,6 +21,61 @@ Module Type CLOCKS
       forall x y ck' xc,
         Is_free_in_clock x ck'
         -> Is_free_in_clock x (Con ck' y xc).
+
+  Require Import Coq.Classes.EquivDec.
+  Open Scope bool.
+
+  Fixpoint clock_eq (ck1 ck2: clock) : bool :=
+    match ck1, ck2 with
+    | Cbase, Cbase => true
+    | Con ck1' x1 b1, Con ck2' x2 b2 =>
+      (Pos.eqb x1 x2 && (b1 ==b b2)) && clock_eq ck1' ck2'
+    | _, _ => false
+    end.
+
+  Lemma clock_eq_spec:
+    forall ck1 ck2,
+      clock_eq ck1 ck2 = true <-> ck1 = ck2.
+  Proof.
+    induction ck1, ck2; split; intro HH; auto;
+      try now inversion HH.
+    - inversion HH as [Heq].
+      apply andb_prop in Heq.
+      destruct Heq as (Heq & Hc).
+      apply andb_prop in Heq.
+      destruct Heq as (Hi & Hb).
+      apply Peqb_true_eq in Hi.
+      rewrite equiv_decb_equiv in Hb.
+      apply IHck1 in Hc.
+      subst. rewrite Hb. reflexivity.
+    - inversion HH as [Heq].
+      subst. simpl.
+      rewrite Bool.andb_true_iff.
+      split. 2:now apply IHck1.
+      rewrite Bool.andb_true_iff.
+      split. now apply Pos.eqb_eq.
+      now apply equiv_decb_equiv.
+  Qed.
+
+  Instance clock_EqDec : EqDec clock eq.
+  Proof.
+    intros ck1 ck2. compute.
+    pose proof (clock_eq_spec ck1 ck2) as Heq.
+    destruct (clock_eq ck1 ck2); [left|right].
+    now apply Heq.
+    intro HH. apply Heq in HH.
+    discriminate.
+  Qed.
+
+  Lemma clock_not_in_clock:
+    forall ck x b,
+      ~(ck = Con ck x b).
+  Proof.
+    intros ** Hck.
+    induction ck; try discriminate.
+    injection Hck; intros.
+    apply IHck. now subst b x.
+  Qed.
 
   (** ** Well-clocking *)
 
@@ -30,6 +88,8 @@ Module Type CLOCKS
         In (x, ck) vars ->
         wc_clock vars (Con ck x b).
 
+  Hint Constructors wc_clock : lclocking.
+
   Definition wc_env vars : Prop :=
     Forall (fun xck => wc_clock vars (snd xck)) vars.
 
@@ -40,7 +100,7 @@ Module Type CLOCKS
       -> wc_clock vars ck.
   Proof.
     intros vars x ck Hwc Hcv.
-    now apply In_Forall with (2:=Hcv) in Hwc.
+    eapply Forall_forall in Hwc; eauto; auto.
   Qed.
 
   Lemma wc_clock_add:
@@ -64,10 +124,10 @@ Module Type CLOCKS
     intros ** Hnm Hwc Hwce.
     constructor.
     now apply wc_clock_add; auto.
-    apply all_In_Forall.
+    apply Forall_forall.
     destruct x0 as (x' & ck').
     intro Hin.
-    apply In_Forall with (1:=Hwce) in Hin.
+    eapply Forall_forall in Hin; eauto.
     apply wc_clock_add; auto.
   Qed.
 
@@ -81,9 +141,6 @@ Module Type CLOCKS
     inversion_clear Hclock as [|? ? ? Hclock' Hcv'].
     assumption.
   Qed.
-
-  Require Import Morphisms.
-  Import Permutation.
 
   Instance wc_clock_Proper:
     Proper (@Permutation (ident * clock) ==> @eq clock ==> iff) wc_clock.
@@ -104,17 +161,29 @@ Module Type CLOCKS
     intros env' env Henv.
     unfold wc_env.
     split; intro HH.
-    - apply all_In_Forall.
+    - apply Forall_forall.
       intros x Hin.
       rewrite <-Henv in Hin.
-      apply In_Forall with (1:=HH) in Hin.
-      now rewrite Henv in Hin.
-    - apply all_In_Forall.
+      eapply Forall_forall in HH; eauto.
+      now rewrite <-Henv.
+    - apply Forall_forall.
       intros x Hin.
       rewrite Henv in Hin.
-      apply In_Forall with (1:=HH) in Hin.
-      now rewrite <-Henv in Hin.
+      eapply Forall_forall in HH; eauto.
+      now rewrite Henv.
   Qed.
+
+  (** ** Instantiate variable clocks from a base clock and substitution *)
+  Fixpoint instck (bk: clock) (sub: ident -> option ident) (ck: clock)
+                                                             : option clock :=
+    match ck with
+    | Cbase => Some bk
+    | Con ck x b => match instck bk sub ck, sub x with
+                    | Some ck', Some x' => Some (Con ck' x' b)
+                    | _, _ => None
+                    end
+    end.
+
 
   (** ** Parent relation *)
 
@@ -148,6 +217,21 @@ Module Type CLOCKS
     inversion Hcp as [|? ? ? Hcp']; [now auto|].
     apply clock_parent_parent' in Hcp'; auto.
   Qed.
+
+  Lemma clock_parent_trans:
+    forall ck1 ck2 ck3,
+      clock_parent ck1 ck2 ->
+      clock_parent ck2 ck3 ->
+      clock_parent ck1 ck3.
+  Proof.
+    induction ck2. now inversion 1.
+    intros ck3 H12 H23.
+    apply clock_parent_parent' in H23.
+    inversion_clear H12; auto.
+  Qed.
+
+  Instance clock_parent_Transitive: Transitive clock_parent.
+  Proof clock_parent_trans.
 
   Lemma clock_parent_Cbase:
     forall ck i b,
@@ -262,6 +346,227 @@ Module Type CLOCKS
     - subst.
       apply IH with (1:=Hwc) (2:=Hp').
       now inversion Hck.
+  Qed.
+
+  Lemma instck_parent:
+    forall bk sub ck ck',
+      instck bk sub ck = Some ck' ->
+      ck' = bk \/ clock_parent bk ck'.
+  Proof.
+    induction ck.
+    now inversion_clear 1; auto.
+    simpl. intros ck' Hi. right.
+    destruct (instck bk sub ck). 2:discriminate.
+    destruct (sub i). 2:discriminate.
+    specialize (IHck c eq_refl).
+    inversion_clear Hi.
+    destruct IHck; subst; auto.
+  Qed.
+
+  (* TODO: move elsewhere *)
+  Lemma instck_subclock_not_clock_eq:
+    forall ck isub xck c x b,
+      instck ck isub xck = Some c ->
+      clock_eq ck (Con c x b) = false.
+  Proof.
+    intros ** Hck.
+    apply Bool.not_true_is_false.
+    intro Heq. apply clock_eq_spec in Heq.
+    apply instck_parent in Hck as [Hck|Hck].
+    now subst c; apply clock_not_in_clock in Heq.
+    now subst ck; apply Con_not_clock_parent in Hck.
+  Qed.
+
+  (* Named clocks *)
+
+  (* Named clocks, as opposed to (stream) clocks, are used to track
+     interdependencies in clock annotations internal to expressions. *)
+
+  Inductive ckid : Type :=
+  | Vidx : positive -> ckid     (* fresh clock *)
+  | Vnm  : ident    -> ckid.    (* named clock *)
+
+  Inductive sclock : Type :=
+  | Sbase : sclock                            (* base clock *)
+  | Son   : sclock -> ckid -> bool -> sclock. (* subclock *)
+
+  Inductive nclock : Type :=
+  | Cstream : sclock -> nclock             (* (unnamed) stream clock *)
+  | Cnamed  : ckid -> sclock -> nclock.    (* named clock: (c : s) or (i : s) *)
+
+  Fixpoint sclk (ck: clock) : sclock :=
+    match ck with
+    | Cbase => Sbase
+    | Con ck x b => Son (sclk ck) (Vnm x) b
+    end.
+
+  Inductive wc_sclock (vars: list (ident * clock)) : sclock -> Prop :=
+  | CSbase:
+      wc_sclock vars Sbase
+  | CSonI:
+      forall sck i b,
+        wc_sclock vars sck ->
+        wc_sclock vars (Son sck (Vidx i) b)
+  | CSonN:
+      forall sck ck x b,
+        wc_sclock vars sck ->
+        In (x, ck) vars ->
+        sck = sclk ck ->
+        wc_sclock vars (Son sck (Vnm x) b).
+
+  Hint Constructors wc_sclock : lclocking.
+
+  Inductive Is_index_in_sclock (i: positive) : sclock -> Prop :=
+  | IdxInSon0: forall sck b,
+      Is_index_in_sclock i (Son sck (Vidx i) b)
+  | IdxInSon1: forall sck ni b,
+      Is_index_in_sclock i sck ->
+      Is_index_in_sclock i (Son sck ni b).
+
+  Inductive Is_index_in_nclock (i: positive) : nclock -> Prop :=
+  | IdxInStream: forall sck,
+      Is_index_in_sclock i sck ->
+      Is_index_in_nclock i (Cstream sck)
+  | IdxInNamed1: forall sck,
+      Is_index_in_nclock i (Cnamed (Vidx i) sck)
+  | IdxInNamed2: forall sck ckid,
+      Is_index_in_sclock i sck ->
+      Is_index_in_nclock i (Cnamed ckid sck).
+
+  Definition Is_index_in_nclocks (i: positive) : list nclock -> Prop :=
+    Exists (Is_index_in_nclock i).
+
+  Hint Unfold Is_index_in_nclocks : lclocking.
+
+  Import ListNotations.
+
+  Function indexes (ncks: list nclock) : list positive :=
+    match ncks with
+    | [] => []
+    | Cnamed (Vidx i) _ :: ncks => i :: indexes ncks
+    | _ :: ncks => indexes ncks
+    end.
+
+  Inductive DisjointIndexes : list (list nclock) -> Prop :=
+  | DisjointIdxNil:
+      DisjointIndexes nil
+  | DisjointIdxCons: forall ncks nckss,
+      DisjointIndexes nckss ->
+      (forall i, Is_index_in_nclocks i ncks ->
+                 Forall (fun ncks' => ~Is_index_in_nclocks i ncks') nckss) ->
+      DisjointIndexes (ncks :: nckss).
+
+  Definition stripname (ck: nclock) : sclock :=
+    match ck with
+    | Cstream sck => sck
+    | Cnamed _ sck => sck
+    end.
+
+  Fixpoint sclock_eq (ck1 ck2: sclock) : bool :=
+    match ck1, ck2 with
+    | Sbase, Sbase => true
+    | Son ck1' (Vnm x1) b1, Son ck2' (Vnm x2) b2 =>
+      (Pos.eqb x1 x2 && (b1 ==b b2)) && sclock_eq ck1' ck2'
+    | Son ck1' (Vidx i1) b1, Son ck2' (Vidx i2) b2 =>
+      (Pos.eqb i1 i2 && (b1 ==b b2)) && sclock_eq ck1' ck2'
+    | _, _ => false
+    end.
+
+  Lemma sclock_eq_spec:
+    forall ck1 ck2,
+      sclock_eq ck1 ck2 = true <-> ck1 = ck2.
+  Proof.
+    induction ck1, ck2; split; intro HH; auto;
+      try now inversion HH.
+    - inversion HH as [Heq].
+      destruct c; inversion Heq.
+    - inversion HH as [Heq].
+      destruct c, c0; try (now inversion Heq).
+      + apply andb_prop in Heq.
+        destruct Heq as (Heq & Hc).
+        apply andb_prop in Heq.
+        destruct Heq as (Hi & Hb).
+        apply Peqb_true_eq in Hi.
+        rewrite equiv_decb_equiv in Hb.
+        apply IHck1 in Hc.
+        subst. rewrite Hb. reflexivity.
+      + apply andb_prop in Heq.
+        destruct Heq as (Heq & Hc).
+        apply andb_prop in Heq.
+        destruct Heq as (Hi & Hb).
+        apply Peqb_true_eq in Hi.
+        rewrite equiv_decb_equiv in Hb.
+        apply IHck1 in Hc.
+        subst. rewrite Hb. reflexivity.
+    - inversion HH as [Heq].
+      destruct c, c0; try (now inversion Heq).
+      + subst. simpl.
+        rewrite Bool.andb_true_iff.
+        split. 2:now apply IHck1.
+        rewrite Bool.andb_true_iff.
+        split. now apply Pos.eqb_eq.
+        now apply equiv_decb_equiv.
+      + subst. simpl.
+        rewrite Bool.andb_true_iff.
+        split. 2:now apply IHck1.
+        rewrite Bool.andb_true_iff.
+        split. now apply Pos.eqb_eq.
+        now apply equiv_decb_equiv.
+  Qed.
+
+  Instance sclock_EqDec : EqDec sclock eq.
+  Proof.
+    intros ck1 ck2. compute.
+    pose proof (sclock_eq_spec ck1 ck2) as Heq.
+    destruct (sclock_eq ck1 ck2); [left|right].
+    now apply Heq.
+    intro HH. apply Heq in HH.
+    discriminate.
+  Qed.
+
+  Lemma not_Is_index_in_sclk:
+    forall i clk,
+      ~Is_index_in_sclock i (sclk clk).
+  Proof.
+    induction clk; now inversion_clear 1.
+  Qed.
+
+  (** Minor predicates on sclock structure *)
+
+  Inductive Name_only_sclock : sclock -> Prop :=
+  | NameOnlySbase:
+      Name_only_sclock Sbase
+  | NameOnlySck: forall sck n b,
+      Name_only_sclock sck ->
+      Name_only_sclock (Son sck (Vnm n) b).
+
+  Inductive Name_only_core_sclock : sclock -> Prop :=
+  | NameOnlyCore0: forall sck,
+      Name_only_sclock sck ->
+      Name_only_core_sclock sck
+  | NameOnlyCore1: forall sck i b,
+      Name_only_core_sclock sck ->
+      Name_only_core_sclock (Son sck (Vidx i) b).
+
+  Lemma Name_only_sclk:
+    forall ck,
+      Name_only_sclock (sclk ck).
+  Proof.
+    induction ck; simpl; auto using Name_only_sclock.
+  Qed.
+
+  Hint Constructors Name_only_sclock Name_only_core_sclock : name_only_sclock.
+  Hint Resolve Name_only_sclk : name_only_sclock.
+
+  Lemma No_index_in_Name_only_sclock:
+    forall sck,
+      Name_only_sclock sck ->
+      (forall j, ~Is_index_in_sclock j sck).
+  Proof.
+    induction sck. now inversion 2.
+    destruct c; inversion_clear 1.
+    inversion_clear 1.
+    eapply IHsck; eauto.
   Qed.
 
 End CLOCKS.
