NLustre/NLClocking.v
@@ -7,6 +7,7 @@ Require Import Velus.NLustre.NLSyntax.
 Require Import Velus.NLustre.IsFree.
 Require Import Velus.NLustre.Memories.
 Require Import Velus.NLustre.IsDefined.
+Require Import Velus.NLustre.Ordered.
 Require Import List.
 
 (** * Well clocked programs *)
@@ -24,12 +25,14 @@ Module Type NLCLOCKING
        (Import Clks    : CLOCKS    Ids)
        (Import ExprSyn : NLEXPRSYNTAX  Op)
        (Import Syn     : NLSYNTAX  Ids Op Clks ExprSyn)
+       (Import Ord     : ORDERED   Ids Op Clks ExprSyn Syn)
        (Import Mem     : MEMORIES  Ids Op Clks ExprSyn Syn)
        (Import IsD     : ISDEFINED Ids Op Clks ExprSyn Syn Mem)
        (Import IsF     : ISFREE    Ids Op Clks ExprSyn Syn).
 
   Section WellClocked.
 
+    Variable G    : global.
     Variable vars : list (ident * clock).
 
     Inductive wc_lexp : lexp -> clock -> Prop :=
@@ -73,6 +76,23 @@ Module Type NLCLOCKING
           wc_lexp e ck ->
           wc_cexp (Eexp e) ck.
 
+    (* TODO: move to Common *)
+    Definition orelse {A B: Type}
+                      (f: A -> option B) (g: A -> option B) (x: A) : option B :=
+      match f x with
+      | None => g x
+      | r => r
+      end.
+
+    Definition subvar_eq (vo : option ident) (le : lexp) : Prop :=
+      match vo with
+      | Some v => match le with
+                  | Evar x _ => v = x
+                  | _ => False
+                  end
+      | None => True
+      end.
+
     Inductive wc_equation : equation -> Prop :=
     | CEqDef:
         forall x ck ce,
@@ -80,16 +100,21 @@ Module Type NLCLOCKING
           wc_cexp ce ck ->
           wc_equation (EqDef x ck ce)
     | CEqApp:
-        forall xs ck f les,
-          Forall (fun x => In (x, ck) vars) xs ->
-          Forall (fun le => wc_lexp le ck) les ->
-          wc_equation (EqApp xs ck f les None)
-    | CEqReset:
-        forall xs ck f les r,
-          Forall (fun x => In (x, ck) vars) xs ->
-          Forall (fun le => wc_lexp le ck) les ->
-          In (r, ck) vars ->
-          wc_equation (EqApp xs ck f les (Some r))
+        forall xs ck f les r n,
+          find_node f G = Some n ->
+          (exists isub osub,
+              Forall2 (fun xtc le => subvar_eq (isub (fst xtc)) le
+                                  /\ (exists lck, wc_lexp le lck
+                                            /\ instck ck isub (dck xtc) = Some lck))
+                      n.(n_in) les
+              /\ Forall2 (fun xtc x => orelse isub osub (fst xtc) = Some x
+                                   /\ (exists xck, In (x, xck) vars
+                                             /\ instck ck (orelse isub osub)
+                                                      (dck xtc) = Some xck))
+                        n.(n_out) xs
+              /\ (forall x, ~InMembers x n.(n_out) -> osub x = None)) ->
+          (forall y, r = Some y -> In (y, ck) vars) ->
+          wc_equation (EqApp xs ck f les r)
     | CEqFby:
         forall x ck v0 le,
           In (x, ck) vars ->
@@ -98,18 +123,20 @@ Module Type NLCLOCKING
 
   End WellClocked.
 
-  Inductive wc_node : node -> Prop :=
-  | SNode:
-      forall n,
-        wc_env (idck (n.(n_in) ++ n.(n_vars) ++ n.(n_out))) ->
-        Forall (wc_equation (idck (n.(n_in) ++ n.(n_vars) ++ n.(n_out))))
-                                                                    n.(n_eqs) ->
-        Forall (fun xtc=> dck xtc = Cbase) n.(n_in) ->
-        Forall (fun xtc=> dck xtc = Cbase) n.(n_out) ->
-        wc_node n.
+  Definition wc_node (G: global) (n: node) : Prop :=
+    wc_env (idck (n.(n_in))) /\
+    wc_env (idck (n.(n_in) ++ n.(n_out))) /\
+    wc_env (idck (n.(n_in) ++ n.(n_vars) ++ n.(n_out))) /\
+    Forall (wc_equation G (idck (n.(n_in) ++ n.(n_vars) ++ n.(n_out))))
+           n.(n_eqs).
 
-  Definition wc_global G : Prop :=
-    Forall (fun nd=> wc_node nd) G.
+  Inductive wc_global : global -> Prop :=
+  | wc_global_nil:
+      wc_global nil
+  | wc_global_cons: forall n ns,
+      wc_global ns ->
+      wc_node ns n ->
+      wc_global (n::ns).
 
   Inductive Has_clock_eq: clock -> equation -> Prop :=
   | HcEqDef: forall x ck ce,
@@ -120,11 +147,6 @@ Module Type NLCLOCKING
       Has_clock_eq ck (EqFby x ck v0 le).
 
   (** ** Basic properties of clocking *)
-
-  Lemma wc_global_nil: wc_global nil.
-  Proof.
-    apply Forall_nil.
-  Qed.
 
   Lemma wc_clock_lexp:
     forall vars le ck,
@@ -160,9 +182,9 @@ Module Type NLCLOCKING
       apply wc_clock_lexp with (1:=Hwc) (2:=Hck).
   Qed.
 
-  Hint Constructors wc_clock wc_lexp wc_cexp wc_equation wc_node : nlclocking.
-  Hint Unfold wc_env : nlclocking.
-  Hint Resolve wc_global_nil Forall_nil : nlclocking.
+  Hint Constructors wc_clock wc_lexp wc_cexp wc_equation wc_global : nlclocking.
+  Hint Unfold wc_env wc_node : nlclocking.
+  Hint Resolve Forall_nil : nlclocking.
 
   Require Import Morphisms.
   Import Permutation.
@@ -199,21 +221,116 @@ Module Type NLCLOCKING
   Qed.
 
   Instance wc_equation_Proper:
-    Proper (@Permutation (ident * clock) ==> @eq equation ==> iff) wc_equation.
+    Proper (@eq global ==> @Permutation (ident * clock) ==> @eq equation ==> iff)
+           wc_equation.
   Proof.
-    intros env1 env2 Henv eq1 eq2 Heq.
-    rewrite Heq; clear Heq.
+    intros G1 G2 Hg env1 env2 Henv eq1 eq2 Heq.
+    rewrite Heq, Hg; clear Heq Hg.
     split; intro WTeq.
-    - inv WTeq; try rewrite Henv in *; eauto with nlclocking;
-        constructor; auto;
-          match goal with H:Forall _ ?x |- Forall _ ?x =>
-                          apply Forall_impl_In with (2:=H) end;
-          intros; rewrite Henv in *; auto.
-    - inv WTeq; try rewrite <-Henv in *; eauto with nlclocking;
-        constructor; auto;
-          match goal with H:Forall _ ?x |- Forall _ ?x =>
-                          apply Forall_impl_In with (2:=H) end;
-          intros; rewrite <-Henv in *; auto.
+    - inv WTeq; try rewrite Henv in *; eauto with nlclocking.
+      match goal with H: exists isub osub, _ |- _ =>
+        destruct H as (isub & osub & Hin & Hout & Hnos) end.
+      econstructor; eauto.
+      + exists isub, osub; repeat split; auto.
+        * apply Forall2_impl_In with (2:=Hin).
+          destruct 3 as (lck & Hwc & Hi).
+          rewrite Henv in *. eauto.
+        * apply Forall2_impl_In with (2:=Hout).
+          destruct 3 as (lck & Hwc & Hi).
+          rewrite Henv in *. eauto.
+      + now setoid_rewrite <-Henv.
+    - inv WTeq; try rewrite <-Henv in *; eauto with nlclocking.
+      match goal with H: exists isub osub, _ |- _ =>
+        destruct H as (isub & osub & Hin & Hout & Hnos) end.
+      econstructor; eauto.
+      + exists isub, osub; repeat split; auto.
+        * apply Forall2_impl_In with (2:=Hin).
+          destruct 3 as (lck & Hwc & Hi).
+          rewrite <-Henv in *. eauto.
+        * apply Forall2_impl_In with (2:=Hout).
+          destruct 3 as (lck & Hwc & Hi).
+          rewrite <-Henv in *. eauto.
+      + now setoid_rewrite Henv.
+  Qed.
+
+  Lemma wc_global_app_weaken:
+    forall G G',
+      wc_global (G' ++ G) ->
+      wc_global G.
+  Proof.
+    induction G'; auto.
+    inversion_clear 1. auto.
+  Qed.
+
+  Lemma wc_find_node:
+    forall G f node,
+      wc_global G ->
+      find_node f G = Some node ->
+      exists G'' G',
+        G = G'' ++ node :: G' /\ wc_node G' node.
+  Proof.
+    intros ** WCG Hfind.
+    apply find_node_split in Hfind as (G'' & G' & HG).
+    rewrite HG in *.
+    apply wc_global_app_weaken in WCG.
+    inversion_clear WCG. eauto.
+  Qed.
+
+  Lemma wc_equation_global_cons:
+    forall vars nd G eq,
+      Ordered_nodes (nd :: G) ->
+      wc_equation G vars eq ->
+      wc_equation (nd :: G) vars eq.
+  Proof.
+    intros ** OnG WCnG.
+    inversion_clear OnG as [|? ? OG ? HndG].
+    inversion_clear WCnG; eauto using wc_equation.
+    econstructor; eauto.
+    simpl. destruct (ident_eqb nd.(n_name) f) eqn:Hf; auto.
+    apply ident_eqb_eq in Hf.
+    rewrite Hf in *.
+    assert (find_node f G <> None) as Hfind by congruence.
+    apply find_node_Exists in Hfind.
+    apply decidable_Exists_not_Forall in Hfind.
+    - contradiction.
+    - auto using decidable_eq_ident.
+  Qed.
+
+  Lemma wc_equation_global_app:
+    forall vars G' G eq,
+      Ordered_nodes (G' ++ G) ->
+      wc_equation G vars eq ->
+      wc_equation (G' ++ G) vars eq.
+  Proof.
+    induction G'; auto.
+    simpl. intros ** OG WCeq.
+    eapply wc_equation_global_cons in OG; eauto.
+    inv OG. auto.
+  Qed.
+
+  Lemma wc_find_node':
+    forall G f node,
+      Ordered_nodes G ->
+      wc_global G ->
+      find_node f G = Some node ->
+      wc_node G node.
+  Proof.
+    intros ** OG WCG Hfind.
+    induction G as [|n' G IH]. discriminate.
+    simpl in *.
+    destruct (ident_eqb n'.(n_name) f) eqn:Heq.
+    - inv Hfind. inversion_clear WCG as [|? ? WCG' (WCi & WCo & WCv & WCeqs)].
+      constructor; repeat (try split; auto).
+      apply Forall_impl_In with (2:=WCeqs).
+      intros. apply wc_equation_global_cons; auto.
+    - assert (OG' := OG).
+      inversion_clear OG as [|? ? OG'' ? ?].
+      inversion_clear WCG as [|? ? WCG'].
+      specialize (IH OG'' WCG' Hfind).
+      destruct IH as (WCi & WCo & WCv & WCeqs).
+      repeat (try split; auto).
+      apply Forall_impl_In with (2:=WCeqs).
+      intros. apply wc_equation_global_cons; auto.
   Qed.
 
   (** Properties *)
@@ -221,21 +338,21 @@ Module Type NLCLOCKING
   Section Well_clocked.
 
     (** We work under a (valid) clocking environment *)
+    Variable G : global.
     Variable vars : list (ident * clock).
     Variable Hnd : NoDupMembers vars.
     Variable Hwc : wc_env vars.
 
     Lemma wc_equation_not_Is_free_in_clock:
       forall eq x ck,
-        wc_equation vars eq
+        wc_equation G vars eq
         -> Is_defined_in_eq x eq
         -> Has_clock_eq ck eq
         -> ~Is_free_in_clock x ck.
     Proof.
       intros eq x' ck' Hwce Hdef Hhasck Hfree.
       inversion Hwce as [x ck e Hcv Hexp Heq
-                        |xs ck f e Hvars Hexp Heq
-                        |xs ck f e r Hvars Hexp Heq
+                        |xs ck f e r n Hfind HH Heq
                         |x ck v' e Hcv Hexp].
       - subst eq. inv Hdef. inv Hhasck.
         pose proof (wc_env_var _ _ _ Hwc Hcv) as Hclock.
@@ -252,34 +369,36 @@ Module Type NLCLOCKING
           apply clock_parent_not_refl with (1:=Hck).
       - subst eq. rename x' into x. inv Hdef. inv Hhasck.
         match goal with H:List.In x xs |- _ => rename H into Hin end.
-        pose proof (In_Forall _ _ _ Hvars Hin) as Hcv.
-        pose proof (wc_env_var _ _ _ Hwc Hcv) as Hclock.
+        destruct HH as (isub & osub & Hisub & Hosub & Hnos).
+        destruct (Forall2_in_right _ _ _ _ Hosub Hin)
+          as (o & Ho & (Hxeq & xck & Hxck & Hxi)).
+        pose proof (wc_env_var _ _ _ Hwc Hxck) as Hclock.
         apply Is_free_in_clock_self_or_parent in Hfree.
-        destruct Hfree as (ck' & b & [Hck|Hck]).
-        + subst ck.
+        apply instck_parent in Hxi.
+        destruct Hxi as [Hxi|Hxi]; destruct Hfree as (ck' & b & [Hck|Hck]).
+        + subst ck xck.
           apply wc_clock_sub with (1:=Hwc) in Hclock.
-          pose proof (NoDupMembers_det _ _ _ _ Hnd Hcv Hclock) as Hloop.
+          pose proof (NoDupMembers_det _ _ _ _ Hnd Hxck Hclock) as Hloop.
           apply clock_no_loops with (1:=Hloop).
-        + apply wc_clock_parent with (1:=Hwc) (2:=Hck) in Hclock.
+        + subst ck.
+          apply wc_clock_parent with (1:=Hwc) (2:=Hck) in Hclock.
           apply wc_clock_sub with (1:=Hwc) in Hclock.
-          rewrite (NoDupMembers_det _ _ _ _ Hnd Hcv Hclock) in *.
+          rewrite (NoDupMembers_det _ _ _ _ Hnd Hxck Hclock) in *.
           apply clock_parent_parent' in Hck.
           apply clock_parent_not_refl with (1:=Hck).
-      - subst eq. rename x' into x. inv Hdef. inv Hhasck.
-        match goal with H:List.In x xs |- _ => rename H into Hin end.
-        pose proof (In_Forall _ _ _ Hvars Hin) as Hcv.
-        pose proof (wc_env_var _ _ _ Hwc Hcv) as Hclock.
-        apply Is_free_in_clock_self_or_parent in Hfree.
-        destruct Hfree as (ck' & b & [Hck|Hck]).
         + subst ck.
+          apply wc_clock_parent with (1:=Hwc) (2:=Hxi) in Hclock.
+          apply clock_parent_parent' in Hxi.
           apply wc_clock_sub with (1:=Hwc) in Hclock.
-          pose proof (NoDupMembers_det _ _ _ _ Hnd Hcv Hclock) as Hloop.
-          apply clock_no_loops with (1:=Hloop).
-        + apply wc_clock_parent with (1:=Hwc) (2:=Hck) in Hclock.
+          rewrite (NoDupMembers_det _ _ _ _ Hnd Hxck Hclock) in *.
+          apply clock_parent_not_refl with (1:=Hxi).
+        + apply wc_clock_parent with (1:=Hwc) (2:=Hxi) in Hclock.
+          apply wc_clock_parent with (1:=Hwc) (2:=Hck) in Hclock.
           apply wc_clock_sub with (1:=Hwc) in Hclock.
-          rewrite (NoDupMembers_det _ _ _ _ Hnd Hcv Hclock) in *.
+          rewrite (NoDupMembers_det _ _ _ _ Hnd Hxck Hclock) in *.
           apply clock_parent_parent' in Hck.
-          apply clock_parent_not_refl with (1:=Hck).
+          apply clock_parent_trans with (1:=Hck) in Hxi.
+          apply clock_parent_not_refl with (1:=Hxi).
       - subst eq. inv Hdef. inv Hhasck.
         pose proof (wc_env_var _ _ _ Hwc Hcv) as Hclock.
         apply Is_free_in_clock_self_or_parent in Hfree.
@@ -297,7 +416,7 @@ Module Type NLCLOCKING
 
     Corollary wc_EqDef_not_Is_free_in_clock:
       forall x ce ck,
-        wc_equation vars (EqDef x ck ce)
+        wc_equation G vars (EqDef x ck ce)
         -> ~Is_free_in_clock x ck.
     Proof.
       intros x ce ck Hwce Hwt.
@@ -306,8 +425,8 @@ Module Type NLCLOCKING
     Qed.
 
     Corollary wc_EqApp_not_Is_free_in_clock:
-      forall xs f le ck r,
-        wc_equation vars (EqApp xs ck f le r)
+      forall xs f le r ck,
+        wc_equation G vars (EqApp xs ck f le r)
         -> forall x, List.In x xs -> ~Is_free_in_clock x ck.
     Proof.
       intros x f le ck Hwce Hwt y Hinx.
@@ -317,7 +436,7 @@ Module Type NLCLOCKING
 
     Corollary wc_EqFby_not_Is_free_in_clock:
       forall x v0 le ck,
-        wc_equation vars (EqFby x ck v0 le)
+        wc_equation G vars (EqFby x ck v0 le)
         -> ~Is_free_in_clock x ck.
     Proof.
       intros x v0 le ck Hwce Hwt.
@@ -330,14 +449,15 @@ Module Type NLCLOCKING
 End NLCLOCKING.
 
 Module NLClockingFun
-       (Ids     : IDS)
-       (Op      : OPERATORS)
-       (Clks    : CLOCKS    Ids)
-       (ExprSyn : NLEXPRSYNTAX  Op)
-       (Syn     : NLSYNTAX  Ids Op Clks ExprSyn)
-       (Mem     : MEMORIES  Ids Op Clks ExprSyn Syn)
-       (IsD     : ISDEFINED Ids Op Clks ExprSyn Syn Mem)
-       (IsF     : ISFREE    Ids Op Clks ExprSyn Syn)
-       <: NLCLOCKING Ids Op Clks ExprSyn Syn Mem IsD IsF.
-  Include NLCLOCKING Ids Op Clks ExprSyn Syn Mem IsD IsF.
+       (Import Ids     : IDS)
+       (Import Op      : OPERATORS)
+       (Import Clks    : CLOCKS    Ids)
+       (Import ExprSyn : NLEXPRSYNTAX  Op)
+       (Import Syn     : NLSYNTAX  Ids Op Clks ExprSyn)
+       (Import Ord     : ORDERED   Ids Op Clks ExprSyn Syn)
+       (Import Mem     : MEMORIES  Ids Op Clks ExprSyn Syn)
+       (Import IsD     : ISDEFINED Ids Op Clks ExprSyn Syn Mem)
+       (Import IsF     : ISFREE    Ids Op Clks ExprSyn Syn)
+  <: NLCLOCKING Ids Op Clks ExprSyn Syn Ord Mem IsD IsF.
+  Include NLCLOCKING Ids Op Clks ExprSyn Syn Ord Mem IsD IsF.
 End NLClockingFun.
