NLustre/NLClockingSemantics.v
@@ -1,0 +1,830 @@
+Require Import Coq.FSets.FMapPositive.
+Require Import Velus.Common.
+Require Import Velus.Operators.
+Require Import Velus.Clocks.
+Require Import Velus.NLustre.Stream.
+Require Import Velus.NLustre.Ordered.
+Require Import Velus.NLustre.NLExprSyntax.
+Require Import Velus.NLustre.NLSyntax.
+Require Import Velus.NLustre.IsFree.
+Require Import Velus.NLustre.Memories.
+Require Import Velus.NLustre.IsDefined.
+Require Import Velus.NLustre.NLClocking.
+Require Import Velus.NLustre.NLExprSemantics.
+Require Import Velus.NLustre.NLSemantics.
+Require Import List.
+
+(** * Link (static) clocking predicates to (dynamic) semantic model *)
+
+(**
+
+These results confirm the correctness of the clocking predicates wrt the
+semantics. In particular, they are useful for relating static invariants to
+dynamic properties. They hold essentially due to the "additional" clocking
+constraints in the NLustre semantic model.
+
+ *)
+
+Module Type NLCLOCKINGSEMANTICS
+       (Import Ids     : IDS)
+       (Import Op      : OPERATORS)
+       (Import OpAux   : OPERATORS_AUX       Op)
+       (Import Clks    : CLOCKS          Ids)
+       (Import ExprSyn : NLEXPRSYNTAX        Op)
+       (Import Syn     : NLSYNTAX        Ids Op       Clks ExprSyn)
+       (Import Str     : STREAM              Op OpAux)
+       (Import Ord     : ORDERED         Ids Op       Clks ExprSyn Syn)
+       (Import ExprSem : NLEXPRSEMANTICS Ids Op OpAux Clks ExprSyn     Str)
+       (Import Sem     : NLSEMANTICS     Ids Op OpAux Clks ExprSyn Syn Str Ord ExprSem)
+       (Import Mem     : MEMORIES        Ids Op       Clks ExprSyn Syn)
+       (Import IsD     : ISDEFINED       Ids Op       Clks ExprSyn Syn                 Mem)
+       (Import IsF     : ISFREE          Ids Op       Clks ExprSyn Syn)
+       (Import Clkg    : NLCLOCKING      Ids Op       Clks ExprSyn Syn     Ord         Mem IsD IsF).
+
+  Definition clock_match (base: stream bool) (H: history) (xc : ident * clock) : Prop :=
+    forall n,
+      (sem_var_instant (restr_hist H n) (fst xc) absent
+       /\ sem_clock_instant (base n) (restr_hist H n) (snd xc) false)
+      \/
+      (exists c,
+          sem_var_instant (restr_hist H n) (fst xc) (present c)
+          /\ sem_clock_instant (base n) (restr_hist H n) (snd xc) true).
+
+  Section ClockMatch.
+
+    Variables
+      (G: global)
+      (vars: list (ident * clock))
+      (bk: stream bool)
+      (H: history)
+      (Hcm: Forall (clock_match bk H) vars).
+
+    Lemma clock_match_lexp:
+      forall le ck,
+        wc_lexp vars le ck ->
+        forall n v,
+          sem_lexp_instant (bk n) (restr_hist H n) le v ->
+          (sem_lexp_instant (bk n) (restr_hist H n) le absent
+           /\ sem_clock_instant (bk n) (restr_hist H n) ck false)
+          \/
+          (exists c,
+              sem_lexp_instant (bk n) (restr_hist H n) le (present c)
+              /\ sem_clock_instant (bk n) (restr_hist H n) ck true).
+    Proof.
+      induction le.
+      - inversion_clear 1. intros.
+        destruct (bk n); [right|left]; eauto using sem_lexp_instant, sem_clock_instant.
+      - inversion_clear 1. intros.
+        eapply Forall_forall in Hcm; eauto.
+        specialize (Hcm n).
+        destruct Hcm as [(Hv & Hc)|(c & Hv & Hc)]; [left|right];
+          eauto using sem_lexp_instant.
+      - repeat inversion_clear 1;
+          repeat match goal with
+                 | WC: wc_lexp _ _ _, SL: sem_lexp_instant _ _ _ _ |- _ =>
+                   destruct (IHle _ WC _ _ SL) as [(Hv & Hc)|(?c & Hv & Hc)]
+                 | HA: sem_lexp_instant _ _ _ absent,
+                   HP: sem_lexp_instant _ _ _ (present ?cv) |- _ =>
+                   now assert (present cv = absent) by sem_det
+                 end.
+        + right; eauto using sem_lexp_instant, sem_clock_instant.
+        + left; eauto using sem_lexp_instant, sem_clock_instant.
+        + left; eauto using sem_lexp_instant, sem_clock_instant.
+      - repeat inversion_clear 1;
+          repeat match goal with
+                 | WC: wc_lexp _ _ _, SL: sem_lexp_instant _ _ _ _ |- _ =>
+                   destruct (IHle _ WC _ _ SL) as [(Hv & Hc)|(?c & Hv & Hc)]
+                 | HA: sem_lexp_instant _ _ _ absent,
+                   HP: sem_lexp_instant _ _ _ (present ?cv) |- _ =>
+                   now assert (present cv = absent) by sem_det
+                 end.
+        + right; eauto using sem_lexp_instant.
+        + left; eauto using sem_lexp_instant.
+      - repeat inversion_clear 1;
+          repeat match goal with
+                 | WC: wc_lexp _ _ _, SL: sem_lexp_instant _ _ _ _ |- _ =>
+                   destruct (IHle1 _ WC _ _ SL) as [(Hv & Hc)|(?c & Hv & Hc)]
+                 | WC: wc_lexp _ _ _, SL: sem_lexp_instant _ _ _ _ |- _ =>
+                   destruct (IHle2 _ WC _ _ SL) as [(Hv & Hc)|(?c & Hv & Hc)]
+                 | HA: sem_lexp_instant _ _ _ absent,
+                   HP: sem_lexp_instant _ _ _ (present ?cv) |- _ =>
+                   now assert (present cv = absent) by sem_det
+                 end.
+        + right; exists c'; eauto using sem_lexp_instant.
+        + left; eauto using sem_lexp_instant.
+    Qed.
+
+    Corollary clock_match_lexp_contradiction:
+      forall le ck b v,
+        wc_lexp vars le ck ->
+        forall n,
+          sem_lexp_instant (bk n) (restr_hist H n) le v ->
+          sem_clock_instant (bk n) (restr_hist H n) ck b ->
+          (b = true <-> v <> absent).
+    Proof.
+      intros le ck b v WC n Hle Hck.
+      eapply clock_match_lexp with (n:=n) in WC as [(Hle' & Hck')|(v' & Hle' & Hck')];
+        eauto.
+      - apply sem_clock_instant_det with (1:=Hck) in Hck'.
+        apply sem_lexp_instant_det with (1:=Hle) in Hle'.
+        subst; intuition.
+      - apply sem_clock_instant_det with (1:=Hck) in Hck'.
+        apply sem_lexp_instant_det with (1:=Hle) in Hle'.
+        subst; intuition; discriminate.
+    Qed.
+
+    Lemma clock_match_cexp:
+      forall ce ck,
+        wc_cexp vars ce ck ->
+        forall n v,
+          sem_cexp_instant (bk n) (restr_hist H n) ce v ->
+          (sem_cexp_instant (bk n) (restr_hist H n) ce absent
+           /\ sem_clock_instant (bk n) (restr_hist H n) ck false)
+          \/
+          (exists c,
+              sem_cexp_instant (bk n) (restr_hist H n) ce (present c)
+              /\ sem_clock_instant (bk n) (restr_hist H n) ck true).
+    Proof.
+      induction ce.
+      - repeat inversion_clear 1.
+        + repeat match goal with
+                 | WC: wc_cexp _ _ _, SL: sem_cexp_instant _ _ _ _ |- _ =>
+                   destruct (IHce1 _ WC _ _ SL) as [(Hv & Hc)|(?c & Hv & Hc)]
+                 | HA: sem_cexp_instant _ _ _ absent,
+                   HP: sem_cexp_instant _ _ _ (present ?cv) |- _ =>
+                   now assert (present cv = absent) by sem_det
+                 end.
+          right; eexists; split; eauto using sem_cexp_instant. inv Hc; auto.
+        + repeat match goal with
+                 | WC: wc_cexp _ _ _, SL: sem_cexp_instant _ _ _ _ |- _ =>
+                   destruct (IHce2 _ WC _ _ SL) as [(Hv & Hc)|(?c & Hv & Hc)]
+                 | HA: sem_cexp_instant _ _ _ absent,
+                   HP: sem_cexp_instant _ _ _ (present ?cv) |- _ =>
+                   now assert (present cv = absent) by sem_det
+                 end.
+          right; eexists; split; eauto using sem_cexp_instant. inv Hc; auto.
+        + repeat match goal with
+                 | WC: wc_cexp _ _ _, SL: sem_cexp_instant _ _ _ _ |- _ =>
+                   destruct (IHce1 _ WC _ _ SL) as [(Hv & Hc)|(?c & Hv & Hc)]
+                 | HA: sem_cexp_instant _ _ _ absent,
+                   HP: sem_cexp_instant _ _ _ (present ?cv) |- _ =>
+                   now assert (present cv = absent) by sem_det
+                 end.
+          left; split; eauto using sem_cexp_instant.
+          inv Hc; auto. now assert (present c = absent) by sem_det.
+      - repeat inversion_clear 1; [right|left];
+          repeat match goal with
+                 | WC: wc_cexp _ _ _, SL: sem_cexp_instant _ _ _ _ |- _ =>
+                   destruct (IHce1 _ WC _ _ SL) as [(Hv1 & Hc1)|(?c & Hv1 & Hc1)]
+                 | WC: wc_cexp _ _ _, SL: sem_cexp_instant _ _ _ _ |- _ =>
+                   destruct (IHce2 _ WC _ _ SL) as [(Hv2 & Hc2)|(?c & Hv2 & Hc2)]
+                 | HA: sem_cexp_instant _ _ _ absent,
+                   HP: sem_cexp_instant _ _ _ (present ?cv) |- _ =>
+                   now assert (present cv = absent) by sem_det
+                 | Hc: sem_lexp_instant _ _ _ (present ?c),
+                   Ht: sem_cexp_instant _ _ _ (present ?ct),
+                   Hf: sem_cexp_instant _ _ _ (present ?cf),
+                   Hv: val_to_bool ?c = Some ?b |- _ =>
+                   apply (Site_eq _ _ _ _ _ _ _ _ _ Hc Ht Hf) in Hv;
+                     destruct b
+                 end; eauto using sem_cexp_instant.
+      - inversion_clear 1 as [| |? ? Hwc].
+        inversion_clear 1.
+        eapply clock_match_lexp in Hwc; eauto.
+        destruct Hwc as [(Hv & Hc)|(?c & Hv & Hc)]; [left|right];
+          eauto using sem_cexp_instant.
+    Qed.
+
+  End ClockMatch.
+
+  Lemma sem_var_transfer_in:
+    forall (xin : list (ident * (type * clock))) H H' les isub bk lss,
+      Forall2 (fun xtc le => subvar_eq (isub (fst xtc)) le) xin les ->
+      sem_lexps bk H les lss ->
+      sem_vars H' (map fst xin) lss ->
+      forall x y ys,
+        InMembers x xin ->
+        isub x = Some y ->
+        sem_var H y ys ->
+        sem_var H' x ys.
+  Proof.
+    intros ** node H H' les isub bk lss Hsv Hles Hlss x y ys Hin Hsub Hvar n.
+    specialize (Hles n); specialize (Hlss n); specialize (Hvar n); simpl in *.
+    unfold sem_vars_instant in Hlss.
+    rewrite Forall2_map_1 in Hlss.
+    apply InMembers_In in Hin as ((xty, xck) & Hxin).
+    apply Forall2_trans_ex with (1:=Hsv) in Hles. clear Hsv.
+    apply Forall2_Forall2 with (1:=Hles) in Hlss. clear Hles.
+    apply Forall2_in_left with (2:=Hxin) in Hlss
+      as (ls & Hinls & (le & Hinle & Hsveq & Hsls) & Hvls).
+    simpl in *. rewrite Hsub in Hsveq.
+    destruct le; try contradiction. simpl in *; subst.
+    inversion_clear Hsls.
+    assert (ys n = ls) as Hys by sem_det.
+    now rewrite Hys in *.
+  Qed.
+
+  (* Transfer named streams defined within the body of a node ([H']) out into
+     the environment where the node is instantiated ([H]). *)
+  Lemma sem_var_instant_transfer_out:
+    forall (xin : list (ident * (type * clock)))
+           (xout : list (ident * (type * clock)))
+           H H' les ys isub osub bk lss yss,
+      NoDupMembers (xin ++ xout) ->
+      Forall2 (fun xtc le => subvar_eq (isub (fst xtc)) le) xin les ->
+      Forall2 (fun xtc  y => orelse isub osub (fst xtc) = Some y) xout ys ->
+      (forall x, ~InMembers x xout -> osub x = None) ->
+      sem_vars H' (map fst xin) lss ->
+      sem_vars H' (map fst xout) yss ->
+      sem_lexps bk H les lss ->
+      sem_vars H ys yss ->
+      forall x y ys,
+        InMembers x (xin ++ xout) ->
+        orelse isub osub x = Some y ->
+        forall n,
+          sem_var_instant (restr_hist H' n) x ys ->
+          sem_var_instant (restr_hist H  n) y ys.
+  Proof.
+    intros ** Hndup Hsv Hos Hnos Hxin Hxout Hles Hys x y s Hin Hsub n Hxv.
+    specialize (Hxin n). specialize (Hxout n).
+    specialize (Hles n). specialize (Hys n). simpl in *.
+    apply InMembers_app in Hin.
+    destruct Hin as [Hin|Hout].
+    - clear Hxout Hys Hos.
+      apply NoDupMembers_app_InMembers with (2:=Hin) in Hndup.
+      apply Hnos in Hndup.
+      apply InMembers_In in Hin as ((xty & xck) & Hin).
+      unfold sem_lexps_instant in Hles.
+      unfold sem_vars_instant in Hxin.
+      rewrite Forall2_map_1 in Hxin.
+      rewrite Forall2_swap_args in Hles.
+      apply Forall2_trans_ex with (1:=Hxin) in Hles. clear Hxin.
+      rewrite Forall2_swap_args in Hsv.
+      apply Forall2_trans_ex with (1:=Hles) in Hsv. clear Hles.
+      apply Forall2_same in Hsv.
+      eapply Forall_forall in Hsv
+        as (le & Hle & (ls & Hlsin & Hxls & Hlels) & Hsveq); eauto.
+      simpl in *.
+      unfold orelse in Hsub.
+      unfold subvar_eq in Hsveq.
+      destruct (isub x); [|congruence].
+      inv Hsub. destruct le; try contradiction.
+      simpl in Hsveq. subst.
+      inversion_clear Hlels.
+      apply sem_var_instant_det with (1:=Hxv) in Hxls.
+      now rewrite Hxls in *.
+    - clear Hsv Hxin Hles.
+      apply InMembers_In in Hout as ((xty & xck) & Hout).
+      unfold sem_vars_instant in Hxout, Hys.
+      rewrite Forall2_map_1 in Hxout.
+      rewrite Forall2_swap_args in Hys.
+      apply Forall2_trans_ex with (1:=Hxout) in Hys. clear Hxout.
+      rewrite Forall2_swap_args in Hos.
+      apply Forall2_trans_ex with (1:=Hys) in Hos. clear Hys.
+      apply Forall2_same in Hos.
+      eapply Forall_forall in Hos
+        as (z & Hz & (v & Hvin & Hv & Hzv) & Hsub'); eauto.
+      simpl in *.
+      rewrite Hsub in Hsub'; inversion_clear Hsub'.
+      apply sem_var_instant_det with (1:=Hxv) in Hv.
+      now rewrite Hv in *.
+  Qed.
+
+  Lemma sem_var_instant_transfer_out':
+    forall n (xin : list (ident * (type * clock)))
+           (xout : list (ident * (type * clock)))
+           H H' les ys isub osub bk lss yss,
+      NoDupMembers (xin ++ xout) ->
+      Forall2 (fun xtc le => subvar_eq (isub (fst xtc)) le) xin les ->
+      Forall2 (fun xtc  y => orelse isub osub (fst xtc) = Some y) xout ys ->
+      (forall x, ~InMembers x xout -> osub x = None) ->
+      sem_vars_instant (restr_hist H' n) (map fst xin) (lss n) ->
+      sem_vars_instant (restr_hist H' n) (map fst xout) (yss n) ->
+      sem_lexps_instant (bk n) (restr_hist H n) les (lss n) ->
+      sem_vars_instant (restr_hist H n) ys (yss n) ->
+      forall x y ys,
+        InMembers x (xin ++ xout) ->
+        orelse isub osub x = Some y ->
+        sem_var_instant (restr_hist H' n) x ys ->
+        sem_var_instant (restr_hist H  n) y ys.
+  Proof.
+    intros ** Hndup Hsv Hos Hnos Hxin Hxout Hles Hys x y s Hin Hsub Hxv.
+    apply InMembers_app in Hin.
+    destruct Hin as [Hin|Hout].
+    - clear Hxout Hys Hos.
+      apply NoDupMembers_app_InMembers with (2:=Hin) in Hndup.
+      apply Hnos in Hndup.
+      apply InMembers_In in Hin as ((xty & xck) & Hin).
+      unfold sem_lexps_instant in Hles.
+      unfold sem_vars_instant in Hxin.
+      rewrite Forall2_map_1 in Hxin.
+      rewrite Forall2_swap_args in Hles.
+      apply Forall2_trans_ex with (1:=Hxin) in Hles. clear Hxin.
+      rewrite Forall2_swap_args in Hsv.
+      apply Forall2_trans_ex with (1:=Hles) in Hsv. clear Hles.
+      apply Forall2_same in Hsv.
+      eapply Forall_forall in Hsv
+        as (le & Hle & (ls & Hlsin & Hxls & Hlels) & Hsveq); eauto.
+      simpl in *.
+      unfold orelse in Hsub.
+      unfold subvar_eq in Hsveq.
+      destruct (isub x); [|congruence].
+      inv Hsub. destruct le; try contradiction.
+      simpl in Hsveq. subst.
+      inversion_clear Hlels.
+      apply sem_var_instant_det with (1:=Hxv) in Hxls.
+      now rewrite Hxls in *.
+    - clear Hsv Hxin Hles.
+      apply InMembers_In in Hout as ((xty & xck) & Hout).
+      unfold sem_vars_instant in Hxout, Hys.
+      rewrite Forall2_map_1 in Hxout.
+      rewrite Forall2_swap_args in Hys.
+      apply Forall2_trans_ex with (1:=Hxout) in Hys. clear Hxout.
+      rewrite Forall2_swap_args in Hos.
+      apply Forall2_trans_ex with (1:=Hys) in Hos. clear Hys.
+      apply Forall2_same in Hos.
+      eapply Forall_forall in Hos
+        as (z & Hz & (v & Hvin & Hv & Hzv) & Hsub'); eauto.
+      simpl in *.
+      rewrite Hsub in Hsub'; inversion_clear Hsub'.
+      apply sem_var_instant_det with (1:=Hxv) in Hv.
+      now rewrite Hv in *.
+  Qed.
+
+  (* Using the transfer of named streams, also transfer clocks from
+     the interface. *)
+  Lemma sem_clock_instant_transfer_out:
+    forall vars ck sub bk bk' H H' xck yck v n,
+      instck ck sub xck = Some yck ->
+      sem_clock_instant (bk n) (restr_hist H n) ck (bk' n) ->
+      wc_clock vars xck ->
+      sem_clock_instant (bk' n) (restr_hist H' n) xck v ->
+      (forall x y ys,
+          InMembers x vars ->
+          sub x = Some y ->
+          sem_var_instant (restr_hist H' n) x ys ->
+          sem_var_instant (restr_hist H  n) y ys) ->
+      sem_clock_instant (bk n) (restr_hist H n) yck v.
+  Proof.
+    intros ** Hinst Hcks Hwc Hsem Hxv.
+    revert xck ck yck v Hinst Hcks Hwc Hsem.
+    induction xck; simpl in *.
+    - inversion 1; inversion 3; now subst.
+    - intros ck yck v Hinst Hcks Hwc Hsem.
+      destruct (instck ck sub xck) eqn:Hi; try discriminate.
+      destruct (sub i) eqn:Hsi; try discriminate.
+      inv Hinst. inv Hwc.
+      apply In_InMembers in H4.
+      inv Hsem; eauto using sem_clock_instant.
+  Qed.
+
+  (* For variables defined in an environment [H], the semantic constraint
+     ([sem_clocked_vars]) forces the [clock_match] property. *)
+  Lemma sem_clocked_vars_clock_match:
+    forall bk H xcks xss,
+      sem_clocked_vars bk H xcks ->
+      sem_vars H (map fst xcks) xss ->
+      Forall (clock_match bk H) xcks.
+  Proof.
+    intros ** Hsv Hvs. apply Forall_forall. intros (x, xck) Hxin n.
+    specialize (Hsv n); specialize (Hvs n).
+    eapply Forall_forall in Hsv; eauto.
+    unfold sem_vars_instant in Hvs.
+    rewrite Forall2_map_1 in Hvs.
+    apply Forall2_in_left with (2:=Hxin) in Hvs as (xs & ? & Hvs).
+    inversion Hsv as [Ht Hf]. simpl in *.
+    destruct xs.
+    - now intuition.
+    - right.
+      pose proof (ex_intro (fun c=>sem_var_instant _ _ (present c)) _ Hvs) as Hevs.
+      apply Ht in Hevs. eauto.
+  Qed.
+
+  (* Transfer interface variable values onto interface clocks between
+     an external environment ([Hn]) and an internal one ([Hn']). *)
+  Lemma clock_vars_to_sem_clock_instant:
+    forall vars bkn Hn Hn' ss,
+      Forall2 (fun xtc => sem_var_instant Hn (fst xtc)) vars ss ->
+      Forall2 (fun xtc => sem_var_instant Hn' (fst xtc)) vars ss ->
+      wc_env (idck vars) ->
+      forall x (xty: type) xck v,
+        In (x, (xty, xck)) vars ->
+        sem_clock_instant bkn Hn xck v ->
+        sem_clock_instant bkn Hn' xck v.
+  Proof.
+    intros vars bkn Hn Hn' ss HHn HHn' WCenv x xty xck v Hin Hsi.
+    assert (exists xty, In (x, (xty, xck)) vars) as Hin' by eauto.
+    apply In_idck_exists in Hin'.
+    apply wc_env_var with (2:=Hin') in WCenv.
+    clear Hin Hin' xty.
+    apply Forall2_Forall2 with (1:=HHn') in HHn. clear HHn'.
+    revert v Hsi. induction xck.
+    - inversion_clear 1; eauto using sem_clock_instant.
+    - inversion_clear WCenv as [|? ? ? WCx Hin].
+      specialize (IHxck WCx).
+      apply In_idck_exists in Hin as (xty & Hin).
+      apply Forall2_in_left with (2:=Hin) in HHn as (s & Hsin & Hv' & Hv).
+      inversion_clear 1.
+      + econstructor; eauto.
+        assert (s = present c) as Hsc by (eapply sem_var_instant_det; eauto).
+        now subst.
+      + econstructor; eauto.
+        assert (s = absent) as Hsc by (eapply sem_var_instant_det; eauto).
+        now subst.
+      + eapply Son_abs2; eauto.
+        assert (s = present c) as Hsc by (eapply sem_var_instant_det; eauto).
+        now subst.
+  Qed.
+
+
+  Lemma clock_match_node_eqs_reset:
+    forall G,
+      Ordered_nodes G ->
+      wc_global G ->
+      (forall f xss yss,
+          sem_node G f xss yss ->
+          forall bk H n,
+            find_node f G = Some n ->
+            clock_of xss bk ->
+            sem_vars H (map fst n.(n_in)) xss ->
+            sem_vars H (map fst n.(n_out)) yss ->
+            Forall (clock_match bk H) (idck n.(n_in)) ->
+            Forall (clock_match bk H) (idck n.(n_out)))
+      /\
+      (forall bk H eq,
+          sem_equation G bk H eq ->
+          forall iface x ck,
+            NoDupMembers iface ->
+            wc_equation G iface eq ->
+            Is_defined_in_eq x eq ->
+            In (x, ck) iface ->
+            clock_match bk H (x, ck))
+      /\
+      (forall f rs xss yss,
+          sem_reset G f rs xss yss ->
+          forall k bk H node,
+            find_node f G = Some node ->
+            clock_of (mask (all_absent (xss 0)) k rs xss) bk ->
+            sem_vars H (map fst node.(n_in)) (mask (all_absent (xss 0)) k rs xss) ->
+            sem_vars H (map fst node.(n_out)) (mask (all_absent (yss 0)) k rs yss) ->
+            Forall (clock_match bk H) (idck node.(n_in)) ->
+            Forall (clock_match bk H) (idck node.(n_out))).
+  Proof.
+    intros ** Hord WCG; apply sem_node_equation_reset_ind;
+      [intros ?????? Hvar Hexp|
+       intros ???????? Hexps Hvars Hsem|
+       intros ??????????? Hexps Hvars ?? Hsem|
+       intros ???????? Hexp Hvar|
+       intros ???? IH|
+       intros ?????? Hck Hf Hin Hout ????? IH].
+
+    - (* EqDef *)
+      intros iface y yck Hnd Hwc Hdef Hin n.
+      inv Hdef. inv Hwc.
+      match goal with H1:In (x, _) iface, H2:In (x, _) iface |- _ =>
+        apply NoDupMembers_det with (1:=Hnd) (2:=H1) in H2; subst end.
+      specialize (Hvar n). specialize (Hexp n).
+      inv Hexp; match goal with H:_ = xs n |- _ => rewrite <-H in * end; eauto.
+
+    - (* EqApp *)
+      intros IHHsem iface z zck Hndup Hwc Hdef Hiface.
+      (* rename ys into yss, y into ys, z into y, zck into yck. *)
+      inversion_clear Hdef as [|? ? ? ? ? Hyys|].
+      inversion_clear Hsem as [cks' H' ??? node Hco' Hfind Hvi Hvo].
+      specialize (IHHsem _ _ _ Hfind Hco' Hvi Hvo).
+      assert (Hvi' := Hvi).
+      rewrite <-map_fst_idck in Hvi'.
+      eapply sem_clocked_vars_clock_match in Hvi'; eauto.
+      pose proof (IHHsem Hvi') as Hscv'. clear IHHsem.
+      inversion_clear Hwc
+        as [|????? node' Hfind' (isub & osub & Hfai & Hfao & Hfno)|].
+      rewrite Hfind in Hfind'. inv Hfind'.
+
+      assert (forall x y ys,
+                 InMembers x (node'.(n_in) ++ node'.(n_out)) ->
+                 orelse isub osub x = Some y ->
+                 forall n,
+                   sem_var_instant (restr_hist H' n) x ys ->
+                   sem_var_instant (restr_hist H  n) y ys) as Htranso.
+      { eapply sem_var_instant_transfer_out; eauto.
+        - pose proof node'.(n_nodup) as Hnd.
+          rewrite <-Permutation_app_assoc,
+                  (Permutation.Permutation_app_comm node'.(n_in)),
+                  Permutation_app_assoc in Hnd.
+          now apply NoDupMembers_app_r in Hnd.
+        - apply Forall2_impl_In with (2:=Hfai). intuition.
+        - apply Forall2_impl_In with (2:=Hfao). intuition.
+        - intro n; specialize (Hexps n); inv Hexps; eauto.
+      }
+
+      rewrite <-map_fst_idck in Hvo. unfold idck in Hvo. rewrite map_map in Hvo.
+      intro n; specialize (Hvo n); specialize (Hvars n); simpl in *.
+      unfold sem_vars_instant in Hvo.
+      rewrite Forall2_map_1 in Hvo.
+      apply Forall2_swap_args in Hfao.
+      apply Forall2_trans_ex with (1:=Hfao) in Hvo.
+      apply Forall2_swap_args in Hvars.
+      apply Forall2_trans_ex with (1:=Hvo) in Hvars.
+      apply Forall2_same in Hvars.
+      eapply Forall_forall in Hvars
+        as (s & Hin & ((x', (xty, xck)) & Hxin &
+                       (Hoeq & yck' & Hiface' & Hinst) & Hsvx) & Hsvy); eauto.
+      unfold dck in Hinst. simpl in *.
+      apply NoDupMembers_det with (1:=Hndup) (2:=Hiface) in Hiface'.
+      rewrite <-Hiface' in *.
+      unfold idck in *. rewrite Forall_map in Hscv'.
+      eapply Forall_forall in Hscv'; eauto; simpl in Hscv'.
+      apply wc_find_node with (1:=WCG) in Hfind as (G'' & G' & HG' & Hfind).
+      destruct Hfind as (WCi & WCo & WCv & WCeqs).
+      assert (In (x', xck) (idck (node'.(n_in) ++ node'.(n_out)))) as Hxin'
+        by (rewrite idck_app, in_app; right;
+            apply In_idck_exists; eauto).
+      apply wc_env_var with (1:=WCo) in Hxin'.
+      destruct (Hscv' n) as [(Hv & Hc)|(c & Hv & Hc)].
+      + left; split.
+        * apply sem_var_instant_det with (1:=Hsvx) in Hv. now subst.
+        *{ eapply sem_clock_instant_transfer_out
+             with (vars := idck (node'.(n_in) ++ node'.(n_out))); eauto.
+           - clear - Hvi Hco' Hexps.
+             specialize (Hco' n); specialize (Hexps n); inversion_clear Hexps as [???? E|??? E].
+             + assert (cks' n = true) as ->; auto.
+               rewrite <-Hco', present_list_spec; eauto.
+             + assert (cks' n = false) as ->; auto.
+               specialize (Hvi n).
+               apply Forall2_length in Hvi; rewrite map_length, E in Hvi.
+               pose proof (n_ingt0 node') as Length; rewrite Hvi in Length.
+               apply Bool.not_true_is_false; rewrite <-Hco', E.
+               clear - Length.
+               destruct arg; simpl in *. omega.
+               inversion 1; congruence.
+           - now setoid_rewrite InMembers_idck; eauto.
+         }
+      + right. exists c; split.
+        * apply sem_var_instant_det with (1:=Hsvx) in Hv. now subst.
+        *{ eapply sem_clock_instant_transfer_out
+             with (vars := idck (node'.(n_in) ++ node'.(n_out))); eauto.
+           - clear - Hvi Hco' Hexps.
+             specialize (Hco' n); specialize (Hexps n); inversion_clear Hexps as [???? E|??? E].
+             + assert (cks' n = true) as ->; auto.
+               rewrite <-Hco', present_list_spec; eauto.
+             + assert (cks' n = false) as ->; auto.
+               specialize (Hvi n).
+               apply Forall2_length in Hvi; rewrite map_length, E in Hvi.
+               pose proof (n_ingt0 node') as Length; rewrite Hvi in Length.
+               apply Bool.not_true_is_false; rewrite <-Hco', E.
+               clear - Length.
+               destruct arg; simpl in *. omega.
+               inversion 1; congruence.
+           - now setoid_rewrite InMembers_idck; eauto.
+         }
+
+    - (* EqReset *)
+      intros IHHsem iface z zck Hndup Hwc Hdef Hiface n.
+      (* rename ys into yss, y into ys, z into y, zck into yck. *)
+      inversion_clear Hdef as [|? ? ? ? ? Hyys|].
+      inversion_clear Hsem as [???? Hsems].
+      specialize (Hsems (count rs n)).
+
+      inversion_clear Hsems as [cks' H' ??? node Hco' Hfind Hvi Hvo].
+      specialize (IHHsem _ _ _ _ Hfind Hco' Hvi Hvo).
+      assert (Hvi' := Hvi).
+      rewrite <-map_fst_idck in Hvi'.
+      eapply sem_clocked_vars_clock_match in Hvi'; eauto.
+      pose proof (IHHsem Hvi') as Hscv'. clear IHHsem.
+      inversion_clear Hwc
+        as [|????? node' Hfind' (isub & osub & Hfai & Hfao & Hfno)|].
+      rewrite Hfind in Hfind'. inv Hfind'.
+
+      assert (forall x y ys,
+                 InMembers x (node'.(n_in) ++ node'.(n_out)) ->
+                 orelse isub osub x = Some y ->
+                 sem_var_instant (restr_hist H' n) x ys ->
+                 sem_var_instant (restr_hist H  n) y ys) as Htranso.
+      { eapply sem_var_instant_transfer_out'; eauto.
+        - pose proof node'.(n_nodup) as Hnd.
+          rewrite <-Permutation_app_assoc,
+                  (Permutation.Permutation_app_comm node'.(n_in)),
+                  Permutation_app_assoc in Hnd.
+          now apply NoDupMembers_app_r in Hnd.
+        - apply Forall2_impl_In with (2:=Hfai). intuition.
+        - apply Forall2_impl_In with (2:=Hfao). intuition.
+        - instantiate (1 := bk).
+          rewrite mask_transparent; auto.
+          specialize (Hexps n); inv Hexps; eauto.
+        - rewrite mask_transparent; auto.
+      }
+
+      rewrite <-map_fst_idck in Hvo. unfold idck in Hvo. rewrite map_map in Hvo.
+      specialize (Hvo n); specialize (Hvars n); simpl in *.
+      rewrite mask_transparent in Hvo; auto.
+      unfold sem_vars_instant in Hvo.
+      rewrite Forall2_map_1 in Hvo.
+      apply Forall2_swap_args in Hfao.
+      apply Forall2_trans_ex with (1:=Hfao) in Hvo.
+      apply Forall2_swap_args in Hvars.
+      apply Forall2_trans_ex with (1:=Hvo) in Hvars.
+      apply Forall2_same in Hvars.
+      eapply Forall_forall in Hvars
+        as (s & Hin & ((x', (xty, xck)) & Hxin &
+                       (Hoeq & yck' & Hiface' & Hinst) & Hsvx) & Hsvy); eauto.
+      unfold dck in Hinst. simpl in *.
+      apply NoDupMembers_det with (1:=Hndup) (2:=Hiface) in Hiface'.
+      rewrite <-Hiface' in *.
+      unfold idck in *. rewrite Forall_map in Hscv'.
+      eapply Forall_forall in Hscv'; eauto; simpl in Hscv'.
+      apply wc_find_node with (1:=WCG) in Hfind as (G'' & G' & HG' & Hfind).
+      destruct Hfind as (WCi & WCo & WCv & WCeqs).
+      assert (In (x', xck) (idck (node'.(n_in) ++ node'.(n_out)))) as Hxin'
+        by (rewrite idck_app, in_app; right;
+            apply In_idck_exists; eauto).
+      apply wc_env_var with (1:=WCo) in Hxin'.
+      destruct (Hscv' n) as [(Hv & Hc)|(c & Hv & Hc)].
+      + left; split.
+        * apply sem_var_instant_det with (1:=Hsvx) in Hv. now subst.
+        *{ eapply sem_clock_instant_transfer_out
+             with (vars := idck (node'.(n_in) ++ node'.(n_out))); eauto.
+           - clear - Hvi Hco' Hexps.
+             specialize (Hco' n); specialize (Hexps n); inversion_clear Hexps as [???? E|??? E].
+             + rewrite mask_transparent in Hco'; auto.
+               assert (cks' n = true) as ->; auto.
+               rewrite <-Hco', present_list_spec; eauto.
+             + assert (cks' n = false) as ->; auto.
+               specialize (Hvi n).
+               rewrite mask_transparent in Hvi, Hco'; auto.
+               apply Forall2_length in Hvi; rewrite map_length, E in Hvi.
+               pose proof (n_ingt0 node') as Length; rewrite Hvi in Length.
+               apply Bool.not_true_is_false; rewrite <-Hco', E.
+               clear - Length.
+               destruct arg; simpl in *. omega.
+               inversion 1; congruence.
+           - now setoid_rewrite InMembers_idck; eauto.
+         }
+      + right. exists c; split.
+        * apply sem_var_instant_det with (1:=Hsvx) in Hv. now subst.
+        *{ eapply sem_clock_instant_transfer_out
+             with (vars := idck (node'.(n_in) ++ node'.(n_out))); eauto.
+           - clear - Hvi Hco' Hexps.
+             specialize (Hco' n); specialize (Hexps n); inversion_clear Hexps as [???? E|??? E].
+             + assert (cks' n = true) as ->; auto.
+               rewrite mask_transparent in Hco'; auto.
+               rewrite <-Hco', present_list_spec; eauto.
+             + assert (cks' n = false) as ->; auto.
+               specialize (Hvi n).
+               rewrite mask_transparent in Hvi, Hco'; auto.
+               apply Forall2_length in Hvi; rewrite map_length, E in Hvi.
+               pose proof (n_ingt0 node') as Length; rewrite Hvi in Length.
+               apply Bool.not_true_is_false; rewrite <-Hco', E.
+               clear - Length.
+               destruct arg; simpl in *. omega.
+               inversion 1; congruence.
+           - now setoid_rewrite InMembers_idck; eauto.
+       }
+
+    - (* EqFby *)
+      intros ? iface z zck Hnd Hwc Hdef Hin n.
+      inv Hdef; inv Hwc.
+      match goal with H1:In (?y, _) iface, H2:In (?y, _) iface |- _ =>
+        apply NoDupMembers_det with (1:=Hnd) (2:=H1) in H2; subst end.
+      specialize (Hexp n). specialize (Hvar n).
+      unfold fby in Hvar.
+      inv Hexp; match goal with H:_ = ls n |- _ => rewrite <-H in * end; eauto.
+
+    - (* reset *)
+      intro k; destruct (IH k); auto.
+
+    - (* nodes *)
+      intros bk' H' n' Hf' Hck' Hin' Hout' Hcm'.
+      rewrite Hf in Hf'. inv Hf'.
+      apply Forall_forall; unfold idck.
+      intros (x, xck) Hxin.
+      apply In_idck_exists in Hxin as (xty & Hxin). assert (Hxin' := Hxin).
+      apply in_map with (f:=fst), node_output_defined_in_eqs in Hxin.
+      apply Is_defined_in_eqs_In in Hxin as (eq & Heqin & Hxeq).
+      eapply Forall_forall in IH; eauto.
+        (* as (Hsem & IH). *)
+      apply wc_find_node with (1:=WCG) in Hf
+        as (G'' & G' & HG & (WCi & WCo & WCv & WCeqs)).
+      eapply Forall_forall in WCeqs; eauto.
+      assert (NoDupMembers (idck (n'.(n_in) ++ n'.(n_vars) ++ n'.(n_out))))
+        as Hnd by apply NoDupMembers_idck, n_nodup.
+      subst.
+      apply IH with (x:=x) (ck:=xck) in Hnd;
+        try (apply In_idck_exists; exists xty);
+        eauto using wc_equation_global_app,
+                    Ordered_nodes_append, wc_equation_global_cons
+              with datatypes.
+      intro n.
+      specialize (Hin' n); specialize (Hout' n);
+        specialize (Hin n); specialize (Hout n).
+      simpl in *.
+      unfold sem_vars_instant in Hin, Hout, Hin', Hout'.
+      rewrite Forall2_map_1 in Hin', Hout'.
+      apply Forall2_app with (2:=Hout') in Hin'.
+      rewrite Forall2_map_1 in Hin, Hout.
+      assert (Hout2:=Hout).
+      apply Forall2_app with (1:=Hin) in Hout2.
+      apply clock_of_det with (1:=Hck) (n:=n) in Hck'.
+      rewrite Hck' in *.
+      apply Forall2_Forall2 with (1:=Hout) in Hout'.
+      apply Forall2_in_left with (2:=Hxin') in Hout' as (s & Hsin & Hvs & Hvs').
+      destruct (Hnd n) as [(Hv & Hc)|(c & Hv & Hc)].
+      + left. simpl in *. split.
+        * apply sem_var_instant_det with (1:=Hvs) in Hv. now subst.
+        * eapply clock_vars_to_sem_clock_instant
+          with (1:=Hout2) (2:=Hin') in WCo; eauto.
+          eapply in_app; eauto.
+      + right. simpl in *. exists c. split.
+        * apply sem_var_instant_det with (1:=Hvs) in Hv. now subst.
+        * eapply clock_vars_to_sem_clock_instant
+          with (1:=Hout2) (2:=Hin') in WCo; eauto.
+          eapply in_app; eauto.
+  Qed.
+
+
+  (* When a node's inputs match their clocks, then so do its outputs.
+     This is a consequence (by induction throughout the node hierarchy) of
+     the constraints relating streams to their clocks for each case of
+     [sem_equation]. *)
+  Lemma clock_match_node:
+    forall G f xss yss bk H n,
+      Ordered_nodes G ->
+      wc_global G ->
+      sem_node G f xss yss ->
+      find_node f G = Some n ->
+      clock_of xss bk ->
+      sem_vars H (map fst n.(n_in)) xss ->
+      sem_vars H (map fst n.(n_out)) yss ->
+      Forall (clock_match bk H) (idck n.(n_in)) ->
+      Forall (clock_match bk H) (idck n.(n_out)).
+  Proof.
+    intros ??????? Ord WCG; intros.
+    eapply (proj1 (clock_match_node_eqs_reset G Ord WCG)); eauto.
+  Qed.
+
+  (* A "version" of [clock_match_node] for "within" a node. Much of the
+     reasoning from [clock_match_node] is unfortunately repeated here. It's
+     not clear whether this is inevitable or whether there is a smarter way
+     to do the induction (maybe by tweaking [sem_node_mult]). The essential
+     difficulty is that the internal environment ([H]) is existentially
+     quantified for a node, which makes it hard to state the lemma relative
+     to [sem_node], and tedious to "transfer" facts known "outside" a
+     node to facts known "within" it. At the time of writing, there is no
+     determinism lemma for environments constrained by nodes. *)
+  Lemma clock_match_eq:
+    forall G bk H iface x ck eq,
+      Ordered_nodes G ->
+      wc_global G ->
+      NoDupMembers iface ->
+      sem_equation G bk H eq ->
+      wc_equation G iface eq ->
+      Is_defined_in_eq x eq ->
+      In (x, ck) iface ->
+      clock_match bk H (x, ck).
+  Proof.
+    intros ??????? Ord WCG; intros.
+    eapply (proj1 (proj2 (clock_match_node_eqs_reset G Ord WCG))); eauto.
+  Qed.
+
+  Lemma clock_match_eqs:
+    forall G bk H inputs vars eqs,
+      Ordered_nodes G ->
+      wc_global G ->
+      NoDupMembers (inputs ++ vars) ->
+      Forall (sem_equation G bk H) eqs ->
+      Forall (wc_equation G (inputs ++ vars)) eqs ->
+      Permutation.Permutation (vars_defined eqs) (map fst vars) ->
+      forall x xck,
+        In (x, xck) vars ->
+        clock_match bk H (x, xck).
+  Proof.
+    intros G bk H inputs vars eqs OG WCG Hndup Hsem Hwc Hdef x xck Hin.
+    assert (In x (vars_defined eqs)) as Hxin
+        by (now rewrite Hdef; apply in_map with (f:=fst) in Hin).
+    apply Is_defined_in_var_defined, Is_defined_in_eqs_In in Hxin
+      as (eq & Hieq & Hdeq).
+    eapply Forall_forall in Hsem; eauto.
+    eapply Forall_forall in Hwc; eauto.
+    eapply clock_match_eq; eauto.
+    rewrite in_app; auto.
+  Qed.
+
+End NLCLOCKINGSEMANTICS.
+
+Module NLClockingSemanticsFun
+       (Import Ids     : IDS)
+       (Import Op      : OPERATORS)
+       (Import OpAux   : OPERATORS_AUX       Op)
+       (Import Clks    : CLOCKS          Ids)
+       (Import ExprSyn : NLEXPRSYNTAX        Op)
+       (Import Syn     : NLSYNTAX        Ids Op       Clks ExprSyn)
+       (Import Str     : STREAM              Op OpAux)
+       (Import Ord     : ORDERED         Ids Op       Clks ExprSyn Syn)
+       (Import ExprSem : NLEXPRSEMANTICS Ids Op OpAux Clks ExprSyn     Str)
+       (Import Sem     : NLSEMANTICS     Ids Op OpAux Clks ExprSyn Syn Str Ord ExprSem)
+       (Import Mem     : MEMORIES        Ids Op       Clks ExprSyn Syn)
+       (Import IsD     : ISDEFINED       Ids Op       Clks ExprSyn Syn                 Mem)
+       (Import IsF     : ISFREE          Ids Op       Clks ExprSyn Syn)
+       (Import Clkg    : NLCLOCKING      Ids Op       Clks ExprSyn Syn     Ord         Mem IsD IsF)
+<: NLCLOCKINGSEMANTICS Ids Op OpAux Clks ExprSyn Syn Str Ord ExprSem Sem Mem IsD IsF Clkg.
+  Include NLCLOCKINGSEMANTICS Ids Op OpAux Clks ExprSyn Syn Str Ord ExprSem Sem Mem IsD IsF Clkg.
+End NLClockingSemanticsFun.
